\documentclass[12pt]{article}
\usepackage{../../../sty/sols}

\olympiad{\textsf{\textbf{IMO Shortlist 2004}}}

\title{Solutions \olympiad}
\author{Samuel de Araújo Brandão}
\date{\today}

\begin{document}
\maketitle
\preface

\tableofcontents

\clearpage

\section{\textsf{Problems}}
\begin{enumerate}[label={\textbf{\arabic*.}}]
	\item If $a$, $b$ ,$c$ are three positive real numbers such that $ab+bc+ca = 1$, prove that\[ \sqrt[3]{ \frac{1}{a} + 6b} + \sqrt[3]{\frac{1}{b} + 6c} + \sqrt[3]{\frac{1}{c} + 6a } \leq \frac{1}{abc}.  \]
\end{enumerate}

\clearpage

\section{\textsf{Solutions}}

\subsubsection{A5}
\begin{problem}
If $a$, $b$ ,$c$ are three positive real numbers such that $ab+bc+ca = 1$, prove that\[ \sqrt[3]{ \frac{1}{a} + 6b} + \sqrt[3]{\frac{1}{b} + 6c} + \sqrt[3]{\frac{1}{c} + 6a } \leq \frac{1}{abc}.  \]
\end{problem}

\textbf{\textcolor{amber}{First solution}} After homogenizing the inequality, we must prove that

\begin{align*}
	 & \cyc \sqrt[3]{\frac{(ab+bc+ca)^2}{a}+6b(ab+bc+ca)} & =   \\
	 & \cyc \sqrt[3]{\frac{(ab+bc+ca)(7ab+bc+ca)}{a}}     & \le \\
	 & \frac{(ab+bc+ca)^2}{abc}.
\end{align*}
By the Hölder's inequality,
\begin{align*}
	\left(\cyc \sqrt[3]{\frac{(ab+bc+ca)(7ab+bc+ca)}{a}}\right)^3 \le \left(\cyc ab+bc+ca\right)\left(\cyc 7ab+bc+ca\right)\left(\cyc \frac{1}{a}\right).
\end{align*}
Therefore, it suffices to prove the following.
\begin{align*}
	\left(\cyc ab+bc+ca\right)\left(\cyc 7ab+bc+ca\right)\left(\cyc \frac{1}{a}\right) & \le \frac{(ab+bc+ca)^6}{(abc)^3}. & \iff \\
	\frac{24(ab+bc+ca)^3}{abc}                                                         & \le \frac{(ab+bc+ca)^6}{(abc)^3}  & \iff \\
	24(abc)^2                                                                          & \le (ab+bc+ca)^3                  & \iff \\
	2\sqrt[3]{3}(abc)^{\frac{2}{3}}                                                    & \le ab+bc+ca.
\end{align*}
By the AM-GM inequality, $ab+bc+ca \ge 3(abc)^{\frac{2}{3}}$. Hence, we must prove that $3 \ge 2\sqrt[3]{3}$.
Which is true, since $27>24$.

Consequently,
\[
	\frac{1}{abc} \ge \cyc \sqrt[3]{\frac{1}{a} +6b}.
\]

\textbf{\textcolor{amber}{Second solution, \href{https://artofproblemsolving.com/community/c6h30865p23434282}{found by DottedCalculator}}} By the Hölder's inequality,
\begin{align*}
	\left(\cyc \left(\frac{1}{a}+6b\right)\right)\left(\cyc 1\right)^2 & \ge \left(\cyc \sqrt[3]{\frac{1}{a}+6b}\right)^3.
	% \sqrt[3]{54(a+b+c)+9\left(\frac{1}{a}+\frac{1}{b}+\frac{1}{c}\right)} & \ge\cyc \sqrt[3]{\frac{1}{a}+6b}.
\end{align*}
Therefore, it suffices to prove that
\begin{align*}
	\frac{1}{(abc)^3} \ge 54(a+b+c)+9\left(\frac{1}{a}+\frac{1}{b}+\frac{1}{c}\right) \iff
	1 \ge 54(abc)^3(a+b+c) + 9(abc)^2 = \\
	9(abc)^2(6abc(a+b+c)+1)
\end{align*}
since $ab+bc+ca=1$.

\clearpage

By the AM-GM inequality, $\frac{1}{27} \ge (abc)^2$, and by the Titu's Lemma, $a^2b^2+b^2c^2+c^2a^2 \ge \frac{(ab+bc+ca)^2}{3} = \frac{1}{3}$.
Hence, $9(abc)^2 \le \frac{1}{3}$ and $6abc(a+b+c)+1 \le 3$. It happens because
\begin{align*}
	6abc(a+b+c)+1 = 3(ab+bc+ca)^2 -3(a^2b^2+b^2c^2+c^2a^2)+1=4-3(a^2b^2+b^2c^2+c^2a^2).
\end{align*}
Thus,
\begin{align*}
	1 \ge 9(abc)^2(6abc(a+b+c)+1).
\end{align*}
Consequently,
\begin{align*}
	\frac{1}{abc} \ge \cyc \sqrt[3]{\frac{1}{a} +6b}.
\end{align*}

\clearpage

\section{\textsf{References}}\label{sec:references}
\end{document}
